# Activity 3.1 - Regular languages

Reference for math symbols:
<https://www.overleaf.com/learn/latex/List_of_Greek_letters_and_math_symbols>

## Names

- Sebastian Moncada
- Samuel Acevedo

## Exercises

1. Give a recursive definition of the set of strings over $\{a, b\}$ that
   contain at least one $b$ and have an even number of $a$’s before the
   first $b$.
   For example: $aab$, $bab$ and $aaaabbabababa$ are in the set,
   but $abb$, $aaab$ and $aa$ are not

   _**SOLUTION:**_

   **Base case:**
   $ b \in L $

   **Recursive step:**
   If $u \in L$, then $aau$, $ua$, $ub$ $\in L$

   **Closure:**
   $ b \in A $ only if it can be obtained from a finite number of applications of the recursive step

2. Let $X = \{aa, bb\}$ and $Y = \{\lambda, b, ab\}$.

   a. List the strings in set $XY$

   | #   | string         | #   | string | #   | string |
   | --- | -------------- | --- | ------ | --- | ------ |
   | 1   | $aa \ \lambda$ | 2   | $aab$  | 3   | $aaab$ |
   | 4   | $bb \ \lambda$ | 5   | $bbb$  | 6   | $bbab$ |

   b. How many strings of length 6 are there in $X^*$?
   #|string|#|string|#|string
   -|-|-|-|-|-
   1|$aaaaaa$|2|$aaaabb$|3|$aabbaa$
   4|$bbaaaa$|5|$bbbbaa$|6|$bbaabb$
   7|$aabbbb$|8|$bbbbbb$

   There are 8 strings of length 6 in $X^*$

   c. List the strings in set $Y^*$ of length three or less

   | #   | string    | #   | string | #   | string |
   | --- | --------- | --- | ------ | --- | ------ |
   | 1   | $\lambda$ | 2   | $b$    | 3   | $ab$   |
   | 4   | $bb$      | 5   | $bab$  | 6   | $abb$  |
   | 7   | $bbb$     |

   d. List the strings in set $X^*Y^*$ of length four or less

   | #   | string    | #   | string     | #   | string |
   | --- | --------- | --- | ---------- | --- | ------ |
   | 1   | $\lambda$ | 2   | b          | 3   | ab     |
   | 4   | bb        | 5   | bab        | 6   | abb    |
   | 7   | bbb       | 8   | abab       | 9   | babb   |
   | 10  | bbab      | 11  | abbb       | 12  | bbbb   |
   | 13  | aa        | 14  | aa b aa ab | 15  | aabb   |
   | 16  | aaaa      | 17  | aabb       | 18  | bbaa   |

3. Give a recursive definition of the set $\{ a^ib^j | 0 ≤ i ≤ j ≤ 2i\}$

   _**SOLUTION:**_

   **Base case:**
   $a \in X$ and $b \in Y$

   **Recursive step:**
   if $ \text{length}(Y) < \text{length}(X) \times 2$, then $ L = XY $

   **Closure:**
   $ L = XY $ only if it can be obtained from a finite number of applications of the recursive step

4. Let $L$ be the set of strings over $\{a, b\}$ generated by the recursive
   definition

   **I. Basis:** $a \in L$ and $b \in L$

   **II. Recursive Step**: If $u \in L$ then $ua \in L$ and $ub \in L$

   **III. Closure**: A string $u \in L$ only if it can be obtained from the
   basis using a finite number of applications of the recursive step.

   - **a.** List the elements in the sets $L_0, L_1, L_2$

     $L_0 = \{\lambda\}$

     $L_1 = \{a, b\}$

     $L_2 = \{aa, ab, ba, bb\}$

   - **b.** Is the string $bbaaba$ in $L$? If so, trace how it is produced. If not, explain why not.

     $u = a \to L = a$

     $u = b \to L = uL = ba$

     $u = a \to L = uL = aba$

     $u = a \to L = uL = aaba$

     $u = b \to L = uL = baaba$

     $u = b \to L = uL = bbaaba$

     $\square$

   - **c.** Is the string $bbaaaabb$ in $L$? If so, trace how it is produced. If not, explain why not

     $u = b \to L = b$

     $u = b \to L = uL = bb$

     $u = a \to L = uL = abb$

     $u = a \to L = uL = aabb$

     $u = a \to L = uL = aaabb$

     $u = a \to L = uL = aaaabb$

     $u = b \to L = uL = baaaabb$

     $u = b \to L = uL = bbaaaabb$

     $\square$

5. Prove, using induction on the length of a string, that $(w^R)^R = w$ for all
   string $w \in \Sigma$

   _**SOLUTION:**_

   **Basis:**
   $\text{length}(w) = 0$, then $w = \lambda$ and $\lambda ^R = \lambda$

   **Inductive Hypothesis:**
   assume that if $\text{length}(w) = n > 0$, then $w = va$, for some string $v$ with length $n-1$ and $a \in \Sigma$, and $w^R = aw^R$

   **Inductive Step:**

   $w = (w^R)^R$

   $w = (aw^R)^R$

   $w = (av)^R$

   $w  = (av)v^R$

   $w  = a((v)v^R)$

   $w  = a((v)^R)$

   $w  = a(v)^R$

   $w  = aw$

   $w  = w$
